Equivariance almost done, stuck at continuity proof in recursion

Denotational.thy
@@ -1,5 +1,5 @@
 theory Denotational
-  imports Terms Heap "FMap-HOLCF" "FMap-Nominal" "~~/src/HOL/HOLCF/HOLCF"
+  imports Terms Heap "FMap-HOLCF" "FMap-Nominal" "~~/src/HOL/HOLCF/Library/Option_Cpo" "~~/src/HOL/HOLCF/HOLCF"  
 begin
 
 default_sort cpo
@@ -23,7 +23,113 @@ lemma (in cont_pt) perm_cont_simp[simp]: "\<pi> \<bullet> x \<sqsubseteq> \<pi> 
 
 lemmas perm_cont2cont[simp,cont2cont] = cont_compose[OF perm_cont]
 
+lemma perm_bottom[simp,eqvt]: "\<pi> \<bullet> \<bottom> = (\<bottom>::'a::{cont_pt,pcpo})"
+using [[show_sorts]] [[show_types]]
+  proof-
+  have "\<bottom> \<sqsubseteq> -\<pi> \<bullet> (\<bottom>::'a::{cont_pt,pcpo})" by simp
+  thm cont2monofunE[OF perm_cont]
+  hence "\<pi> \<bullet> \<bottom> \<sqsubseteq> \<pi> \<bullet> (-\<pi> \<bullet> (\<bottom>::'a::{cont_pt,pcpo}))" by(rule cont2monofunE[OF perm_cont])
+  hence "\<pi> \<bullet> \<bottom> \<sqsubseteq> (\<bottom>::'a::{cont_pt,pcpo})" by simp
+  thus "\<pi> \<bullet> \<bottom> = (\<bottom>::'a::{cont_pt,pcpo})" by simp
+qed
+
 instance var :: cont_pt  by default auto
+
+(*
+lemma cont_transfer[transfer_rule]: "((cr_fmap ===> cr_fmap) ===> op =) (cont :: (('a \<rightharpoonup> 'b) \<Rightarrow> ('a \<rightharpoonup> 'b)) \<Rightarrow> bool)  (cont :: (('a, 'b::cpo) fmap \<Rightarrow> ('a, 'b) fmap) \<Rightarrow> bool) "
+  apply (rule fun_relI)+
+  apply (erule fun_relE)
+  find_theorems name:fun_rel
+  
+  thm fun_relI
+  unfolding cr_fmap_def
+  apply auto
+  unfolding cont_def
+*)
+
+lemma image_eqvt[eqvt]: "\<pi> \<bullet> (f ` S) = (\<pi> \<bullet> f) ` (\<pi> \<bullet> S)"
+  unfolding permute_set_def permute_fun_def
+  by (auto simp add: image_def)
+
+lemma range_eqvt: "\<pi> \<bullet> range Y = range (\<pi> \<bullet> Y)"
+  unfolding image_eqvt UNIV_eqvt ..
+
+
+instance "fmap" :: (cont_pt, cont_pt) cont_pt
+apply default
+proof(rule contI2, rule monofunI)
+  fix \<pi> m1 m2
+  assume "m1 \<sqsubseteq> (m2 :: ('a, 'b) fmap)"
+  hence "fdom m1 = fdom m2"
+    by (rule fmap_below_dom)
+  show "\<pi> \<bullet> m1 \<sqsubseteq> \<pi> \<bullet> m2"
+  proof (rule fmap_belowI')
+    show "fdom (\<pi> \<bullet> m1) = fdom (\<pi> \<bullet> m2)"
+      using `fdom m1 = fdom m2`
+      by (simp add: fdom_perm del: fdom_perm_rev)
+  next
+    fix x
+    assume "x \<in> fdom (\<pi> \<bullet> m1)" and "x \<in> fdom (\<pi> \<bullet> m2)"
+    moreover
+    obtain x2 where "x = \<pi> \<bullet> x2" by (metis eqvt_bound)
+    ultimately
+    have "x2 \<in> fdom m1" "x2 \<in> fdom m2"
+      using `x \<in> fdom (\<pi> \<bullet> m1)` `x \<in> fdom (\<pi> \<bullet> m2)`
+      by (simp add: fdom_perm mem_permute_iff del: fdom_perm_rev)+
+
+    have "the (lookup (\<pi> \<bullet> m1) x) = \<pi> \<bullet> the (lookup m1 x2)"
+      by (simp add: the_lookup_eqvt[OF `x2 \<in> fdom m1`]  `x = _`)
+    also have "... \<sqsubseteq> \<pi> \<bullet> the (lookup m2 x2)"
+      by -(subst perm_cont_simp, rule fmap_belowE[OF `m1 \<sqsubseteq> m2`])
+    also have "... \<sqsubseteq> the (lookup (\<pi> \<bullet> m2) x)"
+      using `x = _`
+      by (simp add: the_lookup_eqvt[OF `x2 \<in> fdom m2`]  )
+    finally show "the (lookup (\<pi> \<bullet> m1) x) \<sqsubseteq> the (lookup (\<pi> \<bullet> m2) x)".
+  qed
+next
+  fix \<pi> Y
+  assume "chain (Y\<Colon>nat \<Rightarrow> ('a, 'b) fmap)"
+  assume "chain (\<lambda>i. \<pi> \<bullet> Y i)"
+  
+  show "\<pi> \<bullet> (\<Squnion> i. Y i) \<sqsubseteq> (\<Squnion> i. \<pi> \<bullet> Y i) "
+  proof(rule fmap_belowI')
+    show "fdom (\<pi> \<bullet> (\<Squnion> i. Y i)) = fdom (\<Squnion> i. \<pi> \<bullet> Y i)"
+      by (simp add: chain_fdom(2)[OF `chain (\<lambda>i. \<pi> \<bullet> Y i)`] chain_fdom(2)[OF `chain Y`] fdom_perm del: fdom_perm_rev)
+  next
+    fix x
+    assume "x \<in> fdom (\<pi> \<bullet> (\<Squnion> i. Y i))"
+    moreover
+    obtain x2 where "x = \<pi> \<bullet> x2" by (metis eqvt_bound)
+    ultimately
+    have "x2 \<in> fdom (\<Squnion> i. Y i)"
+      using `x \<in> fdom (\<pi> \<bullet> (\<Squnion> i. Y i))` 
+      by (simp add: fdom_perm mem_permute_iff del: fdom_perm_rev)+
+    hence "x2 \<in> fdom (Y 0)"
+      by (simp add: chain_fdom(2)[OF `chain Y`])
+      
+    assume  "x \<in> fdom (\<Squnion> i. \<pi> \<bullet> Y i) "
+    hence "x \<in> fdom (\<pi> \<bullet> Y 0)"
+      by (simp add: chain_fdom(2)[OF `chain (\<lambda>i. \<pi> \<bullet> Y i)`])
+
+    have "the (lookup (\<pi> \<bullet> (\<Squnion> i. Y i)) x) = \<pi> \<bullet> (the (lookup (\<Squnion> i. Y i) x2))"
+      by (simp add: the_lookup_eqvt[OF `x2 \<in> fdom (\<Squnion> i. Y i)`]  `x = _`)
+    also have "... = \<pi> \<bullet> (\<Squnion>i. (the (lookup (Y i) x2)))"
+      by (subst lookup_cont[OF `chain Y` `x2 \<in> fdom (Y 0)`], rule refl)
+    also have "... = (\<Squnion>i. \<pi> \<bullet> (the (lookup (Y i) x2)))"
+      by (rule cont2contlubE[OF perm_cont, OF lookup_chain[OF `chain Y` `x2 \<in> fdom (Y 0)`]])
+    also have "... = (\<Squnion>i. the (lookup (\<pi> \<bullet> (Y i)) x))"
+      using `x2 \<in> fdom (Y 0)` chain_fdom(1)[OF `chain Y`] `x = _`
+      apply (subst the_lookup_eqvt)
+      apply auto
+      done
+    also have "... = the (lookup (\<Squnion>i. \<pi> \<bullet> (Y i)) x)"
+      by (subst lookup_cont[OF `chain (\<lambda>i. \<pi> \<bullet> Y i)` `x \<in> fdom (\<pi> \<bullet> Y 0)`], rule refl)
+    finally
+    have "the (lookup (\<pi> \<bullet> (\<Squnion> i. Y i)) x) = the (lookup (\<Squnion> i. \<pi> \<bullet> Y i) x)" .
+    thus "the (lookup (\<pi> \<bullet> (\<Squnion> i. Y i)) x) \<sqsubseteq> the (lookup (\<Squnion> i. \<pi> \<bullet> Y i) x)" by auto
+  qed
+qed
+
 
 instantiation "cfun" :: (cont_pt, cont_pt) pt
 begin
@@ -36,12 +142,11 @@ begin
   done
 end
 
-(*
+
 lemma Lam_eqvt:
   "cont f \<Longrightarrow> \<pi> \<bullet> Abs_cfun f = Abs_cfun (\<pi> \<bullet> f)"
   unfolding permute_fun_def permute_cfun_def
   by auto
-*)
 
 lemma Cfun_app_eqvt[eqvt]:
   "\<pi> \<bullet> (f \<cdot> x) = (\<pi> \<bullet> f) \<cdot> (\<pi> \<bullet> x)"
@@ -80,16 +185,20 @@ apply (drule cont2monofunE[OF perm_cont, OF is_ubD[rotated]])
   proof (rule is_lubI)
 *)
 
+lemma finite_transfer[transfer_rule]: "(op = ===> op =) finite finite" 
+  unfolding fun_rel_eq by (rule refl)
 
-lemma fmap_extend_eqvt[eqvt]:
-  "\<pi> \<bullet> fmap_extend m1 m2 = fmap_extend (\<pi> \<bullet> m1) (\<pi> \<bullet> m2)"
-apply transfer
-apply perm_simp
+lemma fdom_fmap_bottom: "finite S \<Longrightarrow> fdom (fmap_bottom S) = S"
+  by (transfer, auto simp add: dom_def)
 
-lemma fix_extend_eqvt[eqvt]:
-  "\<pi> \<bullet> fix_extend h nh = fix_extend (\<pi> \<bullet> h) (\<pi> \<bullet> nh)"
-unfolding fix_extend_def
-apply perm_simp
+lemma fmap_bottom_eqvt:
+  "finite S \<Longrightarrow> \<pi> \<bullet> (fmap_bottom S :: ('a::pt, 'b::{cont_pt,pcpo}) fmap) = fmap_bottom (\<pi> \<bullet> S)"
+  by (transfer, perm_simp, rule refl)
+
+lemma fmap_update_eqvt[eqvt]:
+  "\<pi> \<bullet> fmap_update m1 (m2 :: ('a::{cont_pt,cpo}, 'b::{cont_pt,cpo}) fmap) = fmap_update (\<pi> \<bullet> m1) (\<pi> \<bullet> m2)"
+  by (transfer, perm_simp, rule refl)
+
 
 class pure_cpo = Nominal2_Base.pure + cpo
 
@@ -121,11 +230,9 @@ translations
   "_cUpdate f (_cupdbinds b bs)" == "_cUpdate (_cUpdate f b) bs"
   "f(x:\<cdot>=y)" == "CONST cfun_upd f x y"
 
-find_theorems cont "if _ then _ else _ "
-
 
 lemma cfun_upd_eqvt[eqvt]: "p \<bullet> (cfun_upd f (x::'a::{cont_pt,discrete_cpo}) y) = cfun_upd (p \<bullet> f) (p \<bullet> x) (p \<bullet> y)"
-by (auto simp add:permute_cfun_def cfun_eq_iff cfun_upd_def)
+  by (auto simp add:permute_cfun_def cfun_eq_iff cfun_upd_def)
 
 domain Value = Fn (lazy "Value \<rightarrow> Value")
 
@@ -162,10 +269,36 @@ lemma heapToEnv_eqvt[eqvt]:
   "\<pi> \<bullet> heapToEnv h eval = heapToEnv (\<pi> \<bullet> h) (\<pi> \<bullet> eval)"
   by (induct h eval rule:heapToEnv.induct, auto simp add: fmap_upd_eqvt  permute_fun_def)
 
+lemma heapToEnv_fdom[simp]:"fdom (heapToEnv h eval) = fst ` set h"
+  by (induct h eval rule:heapToEnv.induct, auto)
 
-lemma fix_extend_eqvt[eqvt]:
-  "\<pi> \<bullet> fix_extend h nh = fix_extend (\<pi> \<bullet> h) (\<pi> \<bullet> nh)"
-unfolding fix_extend_def
+lemma fmap_bottom_lookup[simp]: "\<lbrakk> x \<in> S ; finite S \<rbrakk> \<Longrightarrow> lookup (fmap_bottom S) x = Some \<bottom>"
+  by (transfer, auto)
+
+definition heapExtend :: "Env \<Rightarrow> heap \<Rightarrow> (Env \<Rightarrow> exp \<Rightarrow> Value)  \<Rightarrow> (var, Value) fmap"
+  where
+  "heapExtend \<rho> h eval = fmap_update \<rho> (fix1 (fmap_bottom (fst ` set h))  (\<Lambda> \<rho>'. heapToEnv h (eval \<rho>')))"
+
+lemma heapExtend_eqvt[eqvt]:
+  "\<pi> \<bullet> heapExtend \<rho> h eval = heapExtend (\<pi> \<bullet> \<rho>) (\<pi> \<bullet> h) (\<pi> \<bullet> eval)"
+unfolding heapExtend_def
+apply (subst fmap_update_eqvt)
+apply (subst fix1_eqvt)
+apply (subst beta_cfun)
+defer
+apply (rule fmap_belowI')
+apply simp
+apply simp
+apply (subst fmap_bottom_eqvt)
+apply simp
+apply (subst Lam_eqvt)
+defer
+apply perm_simp
+apply rule
+(* Goal here: cont (\<lambda>\<rho>'. heapToEnv h (eval \<rho>'))  *)
+
+sorry
+
 
 nominal_primrec
   ESem :: "exp \<Rightarrow> Env \<Rightarrow> Value" ("\<lbrakk> _ \<rbrakk>\<^bsub>_\<^esub>"  [60,60] 60)
@@ -176,7 +309,7 @@ where
 | "\<lbrakk> App e x \<rbrakk>\<^bsub>\<rho>\<^esub> = \<lbrakk> e \<rbrakk>\<^bsub>\<rho>\<^esub> \<down>Fn \<lbrakk> Var x \<rbrakk>\<^bsub>\<rho>\<^esub> "
 | "\<lbrakk> Var x \<rbrakk>\<^bsub>\<rho>\<^esub> = the (lookup \<rho> x)"
 | "set (bn as) \<sharp>* \<rho> \<Longrightarrow>\<lbrakk> Let as body\<rbrakk>\<^bsub>\<rho>\<^esub> = \<lbrakk> Let as body\<rbrakk>\<^bsub>\<lbrace> asToHeap as \<rbrace>\<rho>\<^esub>"
-| "\<lbrace> h \<rbrace>\<rho> = fix_extend \<rho> (\<lambda> \<rho>'. heapToEnv h (\<lambda> e . \<lbrakk>e\<rbrakk>\<^bsub>\<rho>'\<^esub>))"
+| "\<lbrace> h \<rbrace>\<rho> = heapExtend \<rho> h (\<lambda> \<rho>' e . \<lbrakk>e\<rbrakk>\<^bsub>\<rho>'\<^esub>)"
 proof-
 have eqvt_at_ESem: "\<And> a b . eqvt_at ESem_HSem_sumC (Inl (a, b)) \<Longrightarrow> eqvt_at (\<lambda>(a, b). ESem a b) (a, b)" sorry
 have eqvt_at_HSem: "\<And> a b . eqvt_at ESem_HSem_sumC (Inr (a, b)) \<Longrightarrow> eqvt_at (\<lambda>(a, b). HSem a b) (a, b)" sorry
